src/UntypedComp8.v
@@ -1,0 +1,261 @@
+Require Import Common.
+
+Require Import Utopia.
+Require Import Metadata.
+Require Import Program.
+
+Require Import ListLemmas.
+Require Import Monads.
+Require Import HList.
+Require Import CompilationUnit.
+Require Import Semantics.
+Require Import HighestValues.
+
+Require Untyped7.
+Require Untyped8.
+
+Module A := Untyped7.
+Module B := Untyped8.
+
+
+Definition compile_expr :=
+    let fix go e :=
+        let fix go_list es :=
+            match es with
+            | [] => []
+            | e :: es => go e :: go_list es
+            end in
+        match e with
+        | A.Arg => B.Arg
+        | A.UpVar idx => B.UpVar idx
+        | A.App f a => B.App (go f) (go a)
+        | A.Constr ctor args => B.Constr ctor (go_list args)
+        | A.Close fname free => B.Close fname (go_list free)
+        | A.Elim ty cases target => B.Elim ty (go_list cases) (go target)
+        end in go.
+
+Definition compile_expr_list :=
+    let go := compile_expr in
+    let fix go_list es :=
+        match es with
+        | [] => []
+        | e :: es => go e :: go_list es
+        end in go_list.
+
+Definition compile_genv := compile_expr_list.
+
+
+Inductive I_expr : A.expr -> B.expr -> Prop :=
+| IArg : I_expr (A.Arg) (B.Arg)
+| IUpVar : forall idx, I_expr (A.UpVar idx) (B.UpVar idx)
+| IApp : forall af aa bf ba,
+        I_expr af bf ->
+        I_expr aa ba ->
+        I_expr (A.App af aa) (B.App bf ba)
+| IConstr : forall ctor aargs bargs,
+        Forall2 I_expr aargs bargs ->
+        I_expr (A.Constr ctor aargs) (B.Constr ctor bargs)
+| IClose : forall fname afree bfree,
+        Forall2 I_expr afree bfree ->
+        I_expr (A.Close fname afree) (B.Close fname bfree)
+| IElim : forall ty acases atarget bcases btarget,
+        Forall2 I_expr acases bcases ->
+        I_expr atarget btarget ->
+        I_expr (A.Elim ty acases atarget) (B.Elim ty bcases btarget)
+.
+
+Inductive I_cont : A.cont -> (B.expr -> B.state) -> Prop :=
+| IKAppL : forall ae2 al ak  be2 bl bk,
+        I_expr ae2 be2 ->
+        Forall2 I_expr al bl ->
+        I_cont ak bk ->
+        I_cont (A.KAppL ae2 al ak) (fun v => B.Run (B.App v be2) bl bk)
+| IKAppR : forall ae1 al ak  be1 bl bk,
+        I_expr ae1 be1 ->
+        Forall2 I_expr al bl ->
+        I_cont ak bk ->
+        I_cont (A.KAppR ae1 al ak) (fun v => B.Run (B.App be1 v) bl bk)
+| IKConstr : forall ctor  avs aes al ak  bvs bes bl bk,
+        Forall2 I_expr avs bvs ->
+        Forall2 I_expr aes bes ->
+        Forall2 I_expr al bl ->
+        I_cont ak bk ->
+        I_cont (A.KConstr ctor avs aes al ak)
+               (fun v => B.Run (B.Constr ctor (bvs ++ v :: bes)) bl bk)
+| IKClose : forall fname  avs aes al ak  bvs bes bl bk,
+        Forall2 I_expr avs bvs ->
+        Forall2 I_expr aes bes ->
+        Forall2 I_expr al bl ->
+        I_cont ak bk ->
+        I_cont (A.KClose fname avs aes al ak)
+               (fun v => B.Run (B.Close fname (bvs ++ v :: bes)) bl bk)
+| IKElim : forall ty  acases al ak  bcases bl bk,
+        Forall2 I_expr acases bcases ->
+        Forall2 I_expr al bl ->
+        I_cont ak bk ->
+        I_cont (A.KElim ty acases al ak)
+               (fun v => B.Run (B.Elim ty bcases v) bl bk)
+| IKStop : I_cont A.KStop B.Stop
+.
+
+Inductive I : A.state -> B.state -> Prop :=
+| IRun : forall ae al ak  be bl bk,
+        I_expr ae be ->
+        Forall2 I_expr al bl ->
+        I_cont ak bk ->
+        I (A.Run ae al ak) (B.Run be bl bk)
+| IStop : forall av bv,
+        I_expr av bv ->
+        I (A.Stop av) (B.Stop bv)
+.
+
+
+
+Ltac i_ctor := intros; constructor; eauto.
+Ltac i_lem H := intros; eapply H; eauto.
+
+Lemma I_run_cont : forall av ak bv bk,
+    I_expr av bv ->
+    I_cont ak bk ->
+    I (A.run_cont ak av) (bk bv).
+intros0 IIval IIcont; invc IIcont; simpl; try solve [repeat i_ctor].
+- i_ctor. i_ctor. i_lem Forall2_app.
+- i_ctor. i_ctor. i_lem Forall2_app.
+Qed.
+
+Lemma I_is_value : forall a b,
+    I_expr a b ->
+    A.is_value a ->
+    B.is_value b.
+mut_induction a using A.expr_rect_mut' with
+    (Pl := fun as_ => forall bs,
+        Forall2 I_expr as_ bs ->
+        Forall A.is_value as_ ->
+        Forall B.is_value bs);
+[ intros0 II Aval; invc II; invc Aval.. | ].
+
+- i_ctor.
+- i_ctor.
+
+- i_ctor.
+- i_ctor.
+
+- finish_mut_induction I_is_value using list.
+Qed exporting.
+Hint Resolve I_is_value.
+Hint Resolve I_is_value_list.
+
+Lemma I_is_value' : forall b a,
+    I_expr a b ->
+    B.is_value b ->
+    A.is_value a.
+mut_induction b using B.expr_rect_mut' with
+    (Pl := fun bs => forall as_,
+        Forall2 I_expr as_ bs ->
+        Forall B.is_value bs ->
+        Forall A.is_value as_);
+[ intros0 II Bval; invc II; invc Bval.. | ].
+
+- i_ctor.
+- i_ctor.
+
+- i_ctor.
+- i_ctor.
+
+- finish_mut_induction I_is_value' using list.
+Qed exporting.
+
+Lemma I_isnt_value : forall a b,
+    I_expr a b ->
+    ~ A.is_value a ->
+    ~ B.is_value b.
+intros0 II Hnval. contradict Hnval. eauto using I_is_value'.
+Qed.
+Hint Resolve I_isnt_value.
+
+
+Lemma I_unroll_elim' : forall acase bcase ctor aargs bargs amk_rec bmk_rec idx,
+    I_expr acase bcase ->
+    Forall2 I_expr aargs bargs ->
+    (forall a b, I_expr a b -> I_expr (amk_rec a) (bmk_rec b)) ->
+    I_expr (A.unroll_elim' acase ctor aargs amk_rec idx)
+           (B.unroll_elim' bcase ctor bargs bmk_rec idx).
+first_induction aargs; intros0 IIcase IIargs IImk_rec; invc IIargs; simpl.
+- assumption.
+- break_if.
+  + eapply IHaargs; eauto. repeat i_ctor.
+  + eapply IHaargs; eauto. repeat i_ctor.
+Qed.
+
+Lemma I_unroll_elim : forall acase bcase ctor aargs bargs amk_rec bmk_rec,
+    I_expr acase bcase ->
+    Forall2 I_expr aargs bargs ->
+    (forall a b, I_expr a b -> I_expr (amk_rec a) (bmk_rec b)) ->
+    I_expr (A.unroll_elim acase ctor aargs amk_rec)
+           (B.unroll_elim bcase ctor bargs bmk_rec).
+intros. eapply I_unroll_elim'; auto.
+Qed.
+
+
+Theorem I_sim : forall AE BE a a' b,
+    Forall2 I_expr AE BE ->
+    I a b ->
+    A.sstep AE a a' ->
+    exists b',
+        B.sstep BE b b' /\
+        I a' b'.
+destruct a as [ae al ak | v];
+intros0 Henv II Astep; inv Astep.
+all: invc II.
+all: try on (I_expr _ be), invc.
+
+- fwd eapply Forall2_nth_error_ex as HH; eauto.  destruct HH as (bv & ? & ?).
+  eexists. split. i_lem B.SArg.
+  i_lem I_run_cont.
+
+- fwd eapply Forall2_nth_error_ex as HH; eauto.  destruct HH as (bv & ? & ?).
+  eexists. split. i_lem B.SUpVar.
+  i_lem I_run_cont.
+
+
+- eexists. split. i_lem B.SAppL.
+  i_ctor. i_ctor.
+
+- eexists. split. i_lem B.SAppR.
+  i_ctor. i_ctor.
+
+- on (I_expr _ bf), invc.
+  fwd eapply Forall2_nth_error_ex with (ys := BE) as HH; eauto.
+    destruct HH as (bbody & ? & ?).
+
+  eexists. split. i_lem B.SMakeCall.
+  i_ctor.
+
+
+- on _, invc_using Forall2_3part_inv.
+  eexists. split. i_lem B.SConstrStep.
+  i_ctor. i_ctor.
+
+- eexists. split. i_lem B.SConstrDone.
+  i_lem I_run_cont. i_ctor.
+
+
+- on _, invc_using Forall2_3part_inv.
+  eexists. split. i_lem B.SCloseStep.
+  i_ctor. i_ctor.
+
+- eexists. split. i_lem B.SCloseDone.
+  i_lem I_run_cont. i_ctor.
+
+
+- eexists. split. i_lem B.SElimTarget.
+  i_ctor. i_ctor.
+
+- fwd eapply Forall2_nth_error_ex as HH; eauto.  destruct HH as (bcase & ? & ?).
+  on (I_expr _ btarget), invc.
+
+  eexists. split. i_lem B.SEliminate.
+  + on (constructor_arg_n _ = _), fun H => rewrite H.
+    i_lem Forall2_length.
+  + i_ctor. i_lem I_unroll_elim. i_ctor.
+Qed.
